{- ****THE CODE***


G is the input graph, s is the source vertex, `(uv) is the length of an edge from u to v, and V is the set of
vertices.

Dijkstra(G, s)
  for all u ‚àà V \ {s}, d(u) = ‚àû
  d(s) = 0
  R = {}
  while R ‚â† V
    pick u ‚àâ R with smallest d(u)
    R = R ‚à™ {u}
    for all vertices v adjacent to u
      if d(v) > d(u) + `(u, v)
        d(v) = d(u) + `(u, v)
-}

{- ***THE PROOF***



Let d(v) be the label found by the algorithm and let Œ¥(v) be the shortest path distance from s-to-v. We
want to show that d(v) = Œ¥(v) for every vertex v at the end of the algorithm, showing that the algorithm
correctly computes the distances. We prove this by induction on |R| via the following lemma:

                    ****Lemma: For each x ‚àà R, d(x) = Œ¥(x).*****


Proof by Induction: Base case (|R| = 1): Since R only grows in size, the only time |R| = 1 is when R = {s} and d(s) = 0 = Œ¥(s), which is correct.


Inductive hypothesis: Let u be the last vertex added to R. Let R0 = R‚à™ {u}. Our I.H. is: for each x ‚àà R‚Ä≤, d(x) = Œ¥(x).


Using the I.H.: By the inductive hypothesis, for every vertex in R‚Ä≤ that isn‚Äôt u, we have the correct distance label. We need only show that d(u) = Œ¥(u) to complete the proof.


Suppose for a contradiction that the shortest path from s-to-u is Q and has length
                                  
                                 ùìÅ(Q) < d(u).


Q starts in R‚Ä≤ and at some leaves R‚Ä≤ (to get to u which is not in R‚Ä≤). Let xy be the first edge along Q that leaves R‚Ä≤. Let Qx be the s-to-x subpath of Q. Clearly:

                              ùìÅ(Qx) + ùìÅ(xy) ‚â§ ùìÅ(Q).


Since d(x) is the length of the shortest s-to-x path by the I.H., d(x) ‚â§ `(Qx), giving us

                              d(x) + `(xy) ‚â§ `(Qx).


Since y is adjacent to x, d(y) must have been updated by the algorithm, so

                               d(y) ‚â§ d(x) + `(xy).


Finally, since u was picked by the algorithm, u must have the smallest distance label:

                                     d(u) ‚â§ d(y).

Combining these inequalities in reverse order gives us the contradiction that d(x) < d(x). Therefore, no suCh shorter path Q must exist and so d(u) = Œ¥(u).


This lemma shows the algorithm is correct by ‚Äúapplying‚Äù the lemma for R = V .
-}
